coq/lib/P4cub/Semantics/Static/Typing.v
@@ -3,209 +3,208 @@ Require Import Coq.PArith.BinPos Coq.ZArith.BinInt Coq.NArith.BinNat
         Poulet4.P4cub.Syntax.CubNotations
         Poulet4.P4cub.Semantics.Static.Util.
 From RecordUpdate Require Import RecordSet.
-Import String AllCubNotations Clmt.Notations RecordSetNotations.
+Import Clmt.Notations RecordSetNotations.
 
 (** * Expression typing. *)
 
 Reserved Notation "'`⟨' Δ , Γ ⟩ ⊢ e ∈ τ" (at level 80, no associativity).
 
-Local Open Scope ty_scope.
-Local Open Scope expr_scope.
+Local Open Scope typ_scope.
+Local Open Scope exp_scope.
 
-Inductive type_expr (Δ : nat) (Γ : list Expr.t)
-  : Expr.e -> Expr.t -> Prop :=
+Inductive type_exp (Δ : nat) (Γ : list Typ.t)
+  : Exp.t -> Typ.t -> Prop :=
 | type_bool (b : bool) :
-  `⟨ Δ, Γ ⟩ ⊢ b ∈ Expr.TBool
+  `⟨ Δ, Γ ⟩ ⊢ Exp.Bool b ∈ Typ.Bool
 | type_bit w n :
   BitArith.bound w n ->
-  `⟨ Δ, Γ ⟩ ⊢ w `W n ∈ Expr.TBit w
+  `⟨ Δ, Γ ⟩ ⊢ w `W n ∈ Typ.Bit w
 | type_int w n :
   IntArith.bound w n ->
-  `⟨ Δ, Γ ⟩ ⊢ w `S n ∈ Expr.TInt w
+  `⟨ Δ, Γ ⟩ ⊢ w `S n ∈ Typ.Int w
 | type_varbit m w n :
   (w <= m)%N ->
   BitArith.bound w n ->
-  `⟨ Δ, Γ ⟩ ⊢ Expr.VarBit m w n ∈ Expr.TVarBit m
+  `⟨ Δ, Γ ⟩ ⊢ Exp.VarBit m w n ∈ Typ.VarBit m
 | type_var τ og x :
   nth_error Γ x = Some τ ->
-  t_ok Δ τ ->
-  `⟨ Δ, Γ ⟩ ⊢ Expr.Var τ og x ∈ τ
+  typ_ok Δ τ ->
+  `⟨ Δ, Γ ⟩ ⊢ Exp.Var τ og x ∈ τ
 | type_slice hi lo e w τ :
   (Npos lo <= Npos hi < w)%N ->
   numeric_width w τ ->
   `⟨ Δ, Γ ⟩ ⊢ e ∈ τ ->
-  `⟨ Δ, Γ ⟩ ⊢ Expr.Slice hi lo e ∈ Expr.TBit (Npos hi - Npos lo + 1)%N
+  `⟨ Δ, Γ ⟩ ⊢ Exp.Slice hi lo e ∈ Typ.Bit (Npos hi - Npos lo + 1)%N
 | type_cast τ τ' e :
   proper_cast τ' τ ->
-  t_ok Δ τ ->
+  typ_ok Δ τ ->
   `⟨ Δ, Γ ⟩ ⊢ e ∈ τ' ->
-  `⟨ Δ, Γ ⟩ ⊢ Expr.Cast τ e ∈ τ
+  `⟨ Δ, Γ ⟩ ⊢ Exp.Cast τ e ∈ τ
 | type_uop op τ τ' e :
-  uop_type op τ τ' ->
-  t_ok Δ τ' ->
+  una_type op τ τ' ->
+  typ_ok Δ τ' ->
   `⟨ Δ, Γ ⟩ ⊢ e ∈ τ ->
-  `⟨ Δ, Γ ⟩ ⊢ Expr.Uop τ' op e ∈ τ'
+  `⟨ Δ, Γ ⟩ ⊢ Exp.Uop τ' op e ∈ τ'
 | type_bop op τ₁ τ₂ τ e₁ e₂ :
-  bop_type op τ₁ τ₂ τ ->
-  t_ok Δ τ ->
+  bin_type op τ₁ τ₂ τ ->
+  typ_ok Δ τ ->
   `⟨ Δ, Γ ⟩ ⊢ e₁ ∈ τ₁ ->
   `⟨ Δ, Γ ⟩ ⊢ e₂ ∈ τ₂ ->
-  `⟨ Δ, Γ ⟩ ⊢ Expr.Bop τ op e₁ e₂ ∈ τ
+  `⟨ Δ, Γ ⟩ ⊢ Exp.Bop τ op e₁ e₂ ∈ τ
 | type_index e₁ e₂ w τ :
-  t_ok Δ τ ->
-  `⟨ Δ, Γ ⟩ ⊢ e₁ ∈ Expr.TArray (Z.to_N (BitArith.upper_bound w)) τ ->
-  `⟨ Δ, Γ ⟩ ⊢ e₂ ∈ Expr.TBit w ->
-  `⟨ Δ, Γ ⟩ ⊢ Expr.Index τ e₁ e₂ ∈ τ
+  typ_ok Δ τ ->
+  `⟨ Δ, Γ ⟩ ⊢ e₁ ∈ Typ.Array (Z.to_N (BitArith.upper_bound w)) τ ->
+  `⟨ Δ, Γ ⟩ ⊢ e₂ ∈ Typ.Bit w ->
+  `⟨ Δ, Γ ⟩ ⊢ Exp.Index τ e₁ e₂ ∈ τ
 | type_member τ x e τs b :
   nth_error τs x = Some τ ->
-  t_ok Δ τ ->
-  `⟨ Δ, Γ ⟩ ⊢ e ∈ Expr.TStruct b τs ->
-  `⟨ Δ, Γ ⟩ ⊢ Expr.Member τ x e ∈ τ
+  typ_ok Δ τ ->
+  `⟨ Δ, Γ ⟩ ⊢ e ∈ Typ.Struct b τs ->
+  `⟨ Δ, Γ ⟩ ⊢ Exp.Member τ x e ∈ τ
 | type_lists ls es τ τs :
-  t_ok_lists Δ ls ->
-  type_lists_ok ls τ τs ->
-  Forall2 (type_expr Δ Γ) es τs ->
-  `⟨ Δ, Γ ⟩ ⊢ Expr.Lists ls es ∈ τ
+  typ_ok_lists Δ ls ->
+  type_lst_ok ls τ τs ->
+  Forall2 (type_exp Δ Γ) es τs ->
+  `⟨ Δ, Γ ⟩ ⊢ Exp.Lists ls es ∈ τ
 | type_error err :
-  `⟨ Δ, Γ ⟩ ⊢ Expr.Error err ∈ Expr.TError
-where "'`⟨' Δ , Γ ⟩ ⊢ e ∈ τ" := (type_expr Δ Γ e τ) : type_scope.
+  `⟨ Δ, Γ ⟩ ⊢ Exp.Error err ∈ Typ.Error
+where "'`⟨' Δ , Γ ⟩ ⊢ e ∈ τ" := (type_exp Δ Γ e τ) : type_scope.
 
-Local Close Scope expr_scope.
+Local Close Scope exp_scope.
 Local Open Scope pat_scope.
 
 (** Select-pattern-typing. *)
-Inductive type_pat : Parser.pat -> Expr.t -> Prop :=
-| type_wild t : type_pat Parser.Wild t
+Inductive type_pat : Pat.t -> Typ.t -> Prop :=
+| type_wild t : type_pat Pat.Wild t
 | type_mask p₁ p₂ w :
-  type_pat p₁ (Expr.TBit w) ->
-  type_pat p₂ (Expr.TBit w) ->
-  type_pat (Parser.Mask p₁ p₂) (Expr.TBit w)
+  type_pat p₁ (Typ.Bit w) ->
+  type_pat p₂ (Typ.Bit w) ->
+  type_pat (Pat.Mask p₁ p₂) (Typ.Bit w)
 | type_range p₁ p₂ w :
-  type_pat p₁ (Expr.TBit w) ->
-  type_pat p₂ (Expr.TBit w) ->
-  type_pat (Parser.Range p₁ p₂) (Expr.TBit w)
+  type_pat p₁ (Typ.Bit w) ->
+  type_pat p₂ (Typ.Bit w) ->
+  type_pat (Pat.Range p₁ p₂) (Typ.Bit w)
 | type_pbit w n :
-  type_pat (w PW n) (Expr.TBit w)
+  type_pat (w PW n) (Typ.Bit w)
 | type_pint w z :
-  type_pat (w PS z) (Expr.TInt w)
+  type_pat (w PS z) (Typ.Int w)
 | type_pstruct ps ts :
   Forall2 type_pat ps ts ->
-  type_pat (Parser.Lists ps) (Expr.TStruct false ts).
+  type_pat (Pat.Lists ps) (Typ.Struct false ts).
 Local Close Scope pat_scope.
 
-(** Parser-expression typing. *)
-Variant type_prsrexpr 
-        (total_states : nat) (Δ : nat) (Γ : list Expr.t)
-  : Parser.pt -> Prop :=
-  | type_goto (st : Parser.state_label) :
+(** Parser-expession typing. *)
+Variant type_trns 
+        (total_states : nat) (Δ : nat) (Γ : list Typ.t)
+  : Trns.t -> Prop :=
+  | type_goto st :
     valid_state total_states st ->
-    type_prsrexpr total_states Δ Γ (Parser.Direct st)
+    type_trns total_states Δ Γ (Trns.Direct st)
   | type_select e default cases τ :
     valid_state total_states default ->
     `⟨ Δ, Γ ⟩ ⊢ e ∈ τ ->
     Forall
       (fun '(p,st) => type_pat p τ /\ valid_state total_states st)
       cases ->
-    type_prsrexpr total_states Δ Γ (Parser.Select e default cases).
+    type_trns total_states Δ Γ (Trns.Select e default cases).
 
 (** * Statement typing. *)
-Inductive type_fun_kind
-  (Δ : nat) (Γ : list Expr.t) (fs : fenv) (c : ctx)
-    : Stmt.fun_kind -> list Expr.t -> Expr.params -> Prop :=
+Inductive type_call
+  (Δ : nat) (Γ : list Typ.t) (fs : fenv) (c : ctx)
+    : Call.t -> list Typ.t -> Typ.params -> Prop :=
 | type_call_funct f τs oe params ot :
   fs f = Some (List.length τs, {|paramargs:=params; rtrns:=ot|}) ->
-  predop lvalue_ok oe ->
-  relop (type_expr Δ Γ) oe (option_map (tsub_t (gen_tsub τs)) ot) ->
-  type_fun_kind Δ Γ fs c (Stmt.Funct f τs oe) τs params
+  predop lexpr_ok oe ->
+  relop (type_exp Δ Γ) oe (option_map (tsub_typ (gen_tsub τs)) ot) ->
+  type_call Δ Γ fs c (Call.Funct f τs oe) τs params
 | type_call_action a cargs aa cparams params :
   action_call_ok aa c ->
   aa a = Some (cparams,params) ->
-  Forall2 (type_expr Δ Γ) cargs cparams ->
-  type_fun_kind Δ Γ fs c (Stmt.Action a cargs) [] params
+  Forall2 (type_exp Δ Γ) cargs cparams ->
+  type_call Δ Γ fs c (Call.Action a cargs) [] params
 | type_call_method ei m τs oe params ot extern_insts methods :
   extern_call_ok extern_insts c ->
   extern_insts ei = Some (inl methods) ->
   Field.get m methods = Some (List.length τs, {|paramargs:=params; rtrns:=ot|}) ->
-  predop lvalue_ok oe ->
-  relop (type_expr Δ Γ) oe (option_map (tsub_t (gen_tsub τs)) ot) ->
-  type_fun_kind Δ Γ fs c (Stmt.Method ei m τs oe) τs params.
+  predop lexpr_ok oe ->
+  relop (type_exp Δ Γ) oe (option_map (tsub_typ (gen_tsub τs)) ot) ->
+  type_call Δ Γ fs c (Call.Method ei m τs oe) τs params
+| type_call_inst x exts insts sig params extern_params :
+  apply_instance_ok insts sig c ->
+  List.length extern_params = List.length exts ->
+  insts x = Some (inr (sig,extern_params,params)) ->
+  type_call Δ Γ fs c (Call.Inst x exts) [] params.
 
 Definition type_arg
-  (Δ : nat) (Γ : list Expr.t) : Expr.arg -> Expr.param -> Prop :=
+  (Δ : nat) (Γ : list Typ.t) : Exp.arg -> Typ.param -> Prop :=
   rel_paramarg
-    (type_expr Δ Γ)
-    (fun e τ => `⟨ Δ, Γ ⟩ ⊢ e ∈ τ /\ lvalue_ok e).
+    (type_exp Δ Γ)
+    (fun e τ => `⟨ Δ, Γ ⟩ ⊢ e ∈ τ /\ lexpr_ok e).
 
 Definition type_args
-  (Δ : nat) (Γ : list Expr.t) : Expr.args -> list Expr.param -> Prop :=
+  (Δ : nat) (Γ : list Typ.t) : Exp.args -> list Typ.param -> Prop :=
   Forall2 (type_arg Δ Γ).
 
 Reserved Notation "'`⧼' Δ , Γ , f , c ⧽ ⊢ s ⊣ sig" (at level 80, no associativity).
 
-Local Open Scope stmt_scope.
+Local Open Scope stm_scope.
 
-Inductive type_stmt (Δ : nat) (Γ : list Expr.t) (fs : fenv)
-  : ctx -> Stmt.s -> signal -> Prop :=
+Inductive type_stm (Δ : nat) (Γ : list Typ.t) (fs : fenv)
+  : ctx -> Stm.t -> Signal.t -> Prop :=
 | type_skip c :
-  `⧼ Δ, Γ, fs, c ⧽ ⊢ Stmt.Skip ⊣ Cont
-| type_return c eo :
+  `⧼ Δ, Γ, fs, c ⧽ ⊢ Stm.Skip ⊣ Signal.Cnt
+| type_ret c eo :
   match c, eo with
   | CFunction (Some τ), Some e => `⟨ Δ, Γ ⟩ ⊢ e ∈ τ
   | c, None => return_void_ok c
   | _, _ => False
   end ->
-  `⧼ Δ, Γ, fs, c ⧽ ⊢ Stmt.Return eo ⊣ Return
+  `⧼ Δ, Γ, fs, c ⧽ ⊢ Stm.Ret eo ⊣ Signal.Ret
 | type_exit c :
   exit_ctx_ok c ->
-  `⧼ Δ, Γ, fs, c ⧽ ⊢ Stmt.Exit ⊣ Exit
-| type_transition total_states i e :
-  type_prsrexpr total_states Δ Γ e ->
-  `⧼ Δ, Γ, fs, CParserState total_states i ⧽ ⊢ Stmt.Transition e ⊣ Trans
-| type_assign c τ e₁ e₂ :
-  lvalue_ok e₁ ->
+  `⧼ Δ, Γ, fs, c ⧽ ⊢ Stm.Exit ⊣ Signal.Ext
+| type_trans total_states i e :
+  type_trns total_states Δ Γ e ->
+  `⧼ Δ, Γ, fs, CParserState total_states i ⧽ ⊢ Stm.Trans e ⊣ Signal.Trns
+| type_asgn c τ e₁ e₂ :
+  lexpr_ok e₁ ->
   `⟨ Δ, Γ ⟩ ⊢ e₁ ∈ τ ->
   `⟨ Δ, Γ ⟩ ⊢ e₂ ∈ τ ->
-  `⧼ Δ, Γ, fs, c ⧽ ⊢ e₁ `:= e₂ ⊣ Cont
+  `⧼ Δ, Γ, fs, c ⧽ ⊢ e₁ `:= e₂ ⊣ Signal.Cnt
 | type_fun_call c params τs args fk :
-  type_fun_kind Δ Γ fs c fk τs params ->
-  Forall (t_ok Δ) τs ->
+  type_call Δ Γ fs c fk τs params ->
+  Forall (typ_ok Δ) τs ->
   type_args Δ Γ args (map (tsub_param (gen_tsub τs)) (map snd params)) ->
-  `⧼ Δ, Γ, fs, c ⧽ ⊢ Stmt.Call fk args ⊣ Cont
-| type_apply
-    c extern_args args x extern_params params sig insts :
-  apply_instance_ok insts sig c ->
-  insts x = Some (inr (sig,extern_params,params)) ->
-  type_args Δ Γ args (map snd params) ->
-  `⧼ Δ, Γ, fs, c ⧽ ⊢ Stmt.Apply x extern_args args ⊣ Cont
+  `⧼ Δ, Γ, fs, c ⧽ ⊢ Stm.App fk args ⊣ Signal.Cnt
 | type_invoke eo tbl tbls aa i n :
   tbls tbl = Some n ->
   predop
     (fun e =>
        `⟨ Δ, Γ ⟩ ⊢
-         e ∈ Expr.TStruct
+         e ∈ Typ.Struct
          false
-         [Expr.TBool; Expr.TBool; Expr.TBit (N.of_nat n)])
+         [Typ.Bool; Typ.Bool; Typ.Bit (N.of_nat n)])
     eo ->
-  `⧼ Δ, Γ, fs, CApplyBlock tbls aa i ⧽ ⊢ Stmt.Invoke eo tbl ⊣ Cont
-| type_vardecl c og τ te s sig :
+  `⧼ Δ, Γ, fs, CApplyBlock tbls aa i ⧽ ⊢ Stm.Invoke eo tbl ⊣ Signal.Cnt
+| type_letin c og τ te s sig :
   SumForall
-    (fun τ' => τ' = τ /\ t_ok Δ τ')
+    (fun τ' => τ' = τ /\ typ_ok Δ τ')
     (fun e => `⟨ Δ, Γ ⟩ ⊢ e ∈ τ) te ->
     `⧼ Δ, τ :: Γ, fs, c ⧽ ⊢ s ⊣ sig ->
-    `⧼ Δ, Γ, fs, c ⧽ ⊢ Stmt.Var og te s ⊣ sig
+    `⧼ Δ, Γ, fs, c ⧽ ⊢ `let og := te `in s ⊣ sig
 | type_seq c s₁ s₂ sig :
-  `⧼ Δ, Γ, fs, c ⧽ ⊢ s₁ ⊣ Cont ->
+  `⧼ Δ, Γ, fs, c ⧽ ⊢ s₁ ⊣ Signal.Cnt ->
   `⧼ Δ, Γ, fs, c ⧽ ⊢ s₂ ⊣ sig ->
   `⧼ Δ, Γ, fs, c ⧽ ⊢ s₁ `; s₂ ⊣ sig
 | type_cond c e s₁ s₂ sig₁ sig₂ sig :
-  lub sig₁ sig₂ = Some sig ->
-  `⟨ Δ, Γ ⟩ ⊢ e ∈ Expr.TBool ->
+  Signal.lub sig₁ sig₂ = Some sig ->
+  `⟨ Δ, Γ ⟩ ⊢ e ∈ Typ.Bool ->
   `⧼ Δ, Γ, fs, c ⧽ ⊢ s₁ ⊣ sig₁ ->
   `⧼ Δ, Γ, fs, c ⧽ ⊢ s₂ ⊣ sig₂ ->
-  `⧼ Δ, Γ, fs, c ⧽ ⊢ If e Then s₁ Else s₂ ⊣ sig
-where "'`⧼' Δ , Γ , fs , c ⧽ '⊢' s ⊣ sig" := (type_stmt Δ Γ fs c s sig).
+  `⧼ Δ, Γ, fs, c ⧽ ⊢ `if e `then s₁ `else s₂ ⊣ sig
+where "'`⧼' Δ , Γ , fs , c ⧽ '⊢' s ⊣ sig" := (type_stm Δ Γ fs c s sig).
 
-Local Close Scope stmt_scope.
+Local Close Scope stm_scope.
 
 (** * Control-declaration typing. *)
 
@@ -213,7 +212,7 @@ Local Close Scope stmt_scope.
 Record ctrl_type_env : Set :=
   mk_ctrl_type_env
     { ctype_vars : nat
-    ; ctypes : list Expr.t
+    ; ctypes : list Typ.t
     ; cfuncts : fenv (** available functions. *)
     ; cinsts : ienv  (** available control instances. *)
     ; actns : aenv   (** available action signatures. *)
@@ -226,25 +225,25 @@ Global Instance eta_ctrl_type_env : Settable _ :=
 Reserved Notation "Γ '⊢ᵪ' d '⊣' result"
          (at level 80, no associativity).
 
-Variant ctrldecl_type : Set :=
-  | ctrl_var_type (τ : Expr.t)
-  | ctrl_act_type (action_name : string)
-      (ctrl_params : list Expr.t) (data_params : Expr.params)
-  | ctrl_tbl_type (table_name : string) (number_of_actions : nat).
+Variant ctrl_type : Set :=
+  | ctrl_var_type (τ : Typ.t)
+  | ctrl_act_type (action_name : String.string)
+      (ctrl_params : list Typ.t) (data_params : Typ.params)
+  | ctrl_tbl_type (table_name : String.string) (number_of_actions : nat).
 
 (** Control declaration typing,
     Producing either a new action or table. *)
-Variant type_ctrldecl (Γ : ctrl_type_env)
-  : Control.d -> ctrldecl_type -> Prop :=
+Variant type_ctrl (Γ : ctrl_type_env)
+  : Ctrl.t -> ctrl_type -> Prop :=
   | type_ctrl_var x te τ :
     SumForall
-      (fun τ' => τ' = τ /\ t_ok (ctype_vars Γ) τ')
+      (fun τ' => τ' = τ /\ typ_ok (ctype_vars Γ) τ')
       (fun e  => `⟨ ctype_vars Γ, ctypes Γ ⟩ ⊢ e ∈ τ) te ->
-    Γ ⊢ᵪ Control.Var x te ⊣ ctrl_var_type τ
+    Γ ⊢ᵪ Ctrl.Var x te ⊣ ctrl_var_type τ
   | type_action action_name cparams dparams body sig :
     `⧼ ctype_vars Γ, map snd cparams ++ bind_all dparams (ctypes Γ),
         cfuncts Γ, CAction (actns Γ) (cinsts Γ) ⧽ ⊢ body ⊣ sig ->
-    Γ ⊢ᵪ Control.Action action_name cparams dparams body
+    Γ ⊢ᵪ Ctrl.Action action_name cparams dparams body
       ⊣ ctrl_act_type action_name (map snd cparams) dparams
   | type_table table_name key actions def :
     (** Keys type. *)
@@ -263,20 +262,20 @@ Variant type_ctrldecl (Γ : ctrl_type_env)
          In a (map fst actions)
          /\ exists ctrl_params data_params,
            actns Γ a = Some (ctrl_params, data_params)
-           /\ Forall2 (type_expr (ctype_vars Γ) (ctypes Γ)) es ctrl_params)
+           /\ Forall2 (type_exp (ctype_vars Γ) (ctypes Γ)) es ctrl_params)
       def ->
-    Γ ⊢ᵪ Control.Table
+    Γ ⊢ᵪ Ctrl.Table
       table_name key actions def ⊣ ctrl_tbl_type table_name (List.length actions)
 where "Γ '⊢ᵪ' d '⊣' result"
-  := (type_ctrldecl Γ d result) : type_scope.
+  := (type_ctrl Γ d result) : type_scope.
 
 Local Open Scope climate_scope.
 
-Definition type_ctrl
-           (Γ : list Expr.t)
+Definition type_ctrls
+           (Γ : list Typ.t)
            (fs : fenv)
            (cis : ienv)
-           (ctrl : list Control.d) : ctrl_type_env -> Prop :=
+           (ctrl : list Ctrl.t) : ctrl_type_env -> Prop :=
   FoldLeft
     (fun d Γ Γ' =>
        exists result,
@@ -313,19 +312,19 @@ Reserved Notation "Γ₁ '⊢tp' d ⊣ Γ₂"
          (at level 80, no associativity).
 
 (** Top-level declaration typing. *)
-Inductive type_topdecl (Γ : top_type_env)
-  : TopDecl.d -> top_type_env -> Prop :=
-| type_instantiate_control
-    control_decl_name instance_name
-    cparams expr_cparams cargs expr_cargs extern_params params :
-  cnstrs Γ control_decl_name =
-    Some (ControlType cparams expr_cparams extern_params params) ->
+Inductive type_top (Γ : top_type_env)
+  : Top.t -> top_type_env -> Prop :=
+| type_instantiate_cnstr
+    sig decl_name instance_name
+    cparams exp_cparams cargs exp_cargs extern_params params :
+  cnstrs Γ decl_name =
+    Some (CtrType sig cparams exp_cparams extern_params params) ->
   Forall2
     (fun carg cparam =>
        match cparam with
-       | TopDecl.ControlInstType eps ps
-         => insts_env Γ carg = Some (inr (ControlSig,eps,ps))
-       | TopDecl.ExternInstType extern_type
+       | InstTyp.Ctr sig eps ps
+         => insts_env Γ carg = Some (inr (sig,eps,ps))
+       | InstTyp.Extern extern_type
          => (* TODO:
               How to represent extern types?
               [nth_error (externs (insts_envs Γ)) extn = extern_type] *)
@@ -333,53 +332,25 @@ Inductive type_topdecl (Γ : top_type_env)
        | _ => False
        end) cargs cparams ->
   Forall2
-    (type_expr 0 [])
-    expr_cargs expr_cparams ->
-  Γ ⊢tp TopDecl.Instantiate
-    control_decl_name instance_name [] cargs expr_cargs
+    (type_exp 0 [])
+    exp_cargs exp_cparams ->
+  Γ ⊢tp Top.Instantiate
+    decl_name instance_name [] cargs exp_cargs
     ⊣ Γ <| insts_env :=
     insts_bind_other
-      instance_name ControlSig extern_params params
+      instance_name sig extern_params params
       Γ.(insts_env) |>
-| type_instantiate_parser
-    parser_decl_name instance_name
-    cparams expr_cparams cargs expr_cargs extern_params params :
-  cnstrs Γ parser_decl_name =
-    Some (ParserType cparams expr_cparams extern_params params) ->
-  Forall2
-    (fun carg cparam =>
-       match cparam with
-       | TopDecl.ParserInstType eps ps
-         => insts_env Γ carg = Some (inr (ParserSig,eps,ps))
-       | TopDecl.ExternInstType extern_type
-         => (* TODO:
-              How to represent extern types?
-              [nth_error (externs (insts_envs Γ)) extn = extern_type] *)
-           False
-       | _ => False
-       end) cargs cparams ->
-  Forall2
-    (type_expr 0 [])
-    expr_cargs expr_cparams ->
-  Γ ⊢tp TopDecl.Instantiate
-    parser_decl_name instance_name [] cargs expr_cargs
-    ⊣ Γ <| insts_env :=
-      insts_bind_other
-        instance_name ParserSig extern_params params
-        Γ.(insts_env) |>
 | type_instantiate_package
     package_decl_name instance_name
-    cparams expr_cparams cargs expr_cargs :
+    cparams exp_cparams cargs exp_cargs :
   cnstrs Γ package_decl_name =
-    Some (PackageType cparams expr_cparams) ->
+    Some (PackageType cparams exp_cparams) ->
   Forall2
     (fun carg cparam =>
        match cparam with
-       | TopDecl.ControlInstType eps ps
-         => insts_env Γ carg = Some (inr (ControlSig,eps,ps))
-       | TopDecl.ParserInstType eps ps
-         => insts_env Γ carg = Some (inr (ParserSig,eps,ps))
-       | TopDecl.ExternInstType extern_type
+       | InstTyp.Ctr sig eps ps
+         => insts_env Γ carg = Some (inr (sig,eps,ps))
+       | InstTyp.Extern extern_type
          => (* TODO:
               How to represent extern types?
               [nth_error (externs (insts_envs Γ)) extn = extern_type] *)
@@ -387,98 +358,98 @@ Inductive type_topdecl (Γ : top_type_env)
        | _ => False
        end) cargs cparams ->
   Forall2
-    (type_expr 0 [])
-    expr_cargs expr_cparams ->
-  Γ ⊢tp TopDecl.Instantiate
-    package_decl_name instance_name [] cargs expr_cargs
+    (type_exp 0 [])
+    exp_cargs exp_cparams ->
+  Γ ⊢tp Top.Instantiate
+    package_decl_name instance_name [] cargs exp_cargs
     ⊣ Γ (* TODO: represent package types in [ienv] *)
 | type_instantiate_extern
     (* TODO: How to represent extern types & type instantiations? *)
     extern_decl_name extern_name
-    expr_cparams cparams τs expr_cargs cargs methods :
-  Forall (t_ok 0) τs ->
+    exp_cparams cparams τs exp_cargs cargs methods :
+  Forall (typ_ok 0) τs ->
   cnstrs Γ extern_decl_name =
-    Some (ExternType (List.length τs) cparams expr_cparams extern_name) ->
+    Some (ExternType (List.length τs) cparams exp_cparams extern_name) ->
   Forall2
     (fun carg cparam =>
        match cparam with
-       | TopDecl.ExternInstType extern_type
+       | InstTyp.Extern extern_type
          => (* TODO:
               How to represent extern types?
               [nth_error (externs (insts_envs Γ)) extn = extern_type] *)
            False
        | _ => False
        end)
-    cargs (map (tsub_cparam (gen_tsub τs)) cparams) ->
+    cargs (map (tsub_insttyp (gen_tsub τs)) cparams) ->
   Forall2
-    (type_expr 0 [])
-    expr_cargs (map (tsub_t (gen_tsub τs)) expr_cparams) ->
-  Γ ⊢tp TopDecl.Instantiate extern_decl_name extern_name τs cargs expr_cargs
+    (type_exp 0 [])
+    exp_cargs (map (tsub_typ (gen_tsub τs)) exp_cparams) ->
+  Γ ⊢tp Top.Instantiate extern_decl_name extern_name τs cargs exp_cargs
     ⊣ Γ <| insts_env := (* TODO: sub [τs] into methods *)
          insts_bind_externs
          extern_name methods Γ.(insts_env) |>   
 | type_control
-    control_name cparams expr_cparams extern_params params
+    control_name cparams exp_cparams extern_params params
     control_decls apply_blk Γ' sig insts :
-  (* TODO: check params are [t_ok []] *)
+  (* TODO: check params are [typ_ok []] *)
   (* TODO: add extern runtime params
      to instance envrionment when checking control body. *)
   insts = cbind_all (insts_env Γ) cparams ->
-  type_ctrl
-    expr_cparams (tfuncts Γ) insts control_decls Γ' ->
-  `⧼ 0, bind_all params expr_cparams,
+  type_ctrls
+    exp_cparams (tfuncts Γ) insts control_decls Γ' ->
+  `⧼ 0, bind_all params exp_cparams,
       tfuncts Γ, CApplyBlock (tbls Γ') (actns Γ') insts ⧽
     ⊢ apply_blk ⊣ sig ->
   Γ ⊢tp
-    TopDecl.Control
-    control_name cparams expr_cparams extern_params
+    Top.Control
+    control_name cparams exp_cparams extern_params
     params control_decls apply_blk
     ⊣ Γ <| cnstrs :=
     control_name
-      ↦ ControlType
-      (map snd cparams) expr_cparams (map snd extern_params) params ,, cnstrs Γ |>
+      ↦ CtrType Cnstr.Control
+      (map snd cparams) exp_cparams (map snd extern_params) params ,, cnstrs Γ |>
 | type_parser
-    parser_decl_name cparams expr_cparams extern_params params
+    parser_decl_name cparams exp_cparams extern_params params
     start_state states insts :
-  (* TODO: check params are [t_ok []] *)
+  (* TODO: check params are [typ_ok []] *)
   (* TODO: add extern runtime params
      to instance envrionment when checking control body. *)
   insts = cbind_all (insts_env Γ) cparams ->
   Forall
     (fun state =>
-       `⧼ 0, bind_all params expr_cparams, tfuncts Γ,
-           CParserState (List.length states) insts ⧽ ⊢ state ⊣ Trans)
+       `⧼ 0, bind_all params exp_cparams, tfuncts Γ,
+           CParserState (List.length states) insts ⧽ ⊢ state ⊣ Signal.Trns)
     (start_state :: states) ->
-  Γ ⊢tp TopDecl.Parser
-    parser_decl_name cparams expr_cparams extern_params params
+  Γ ⊢tp Top.Parser
+    parser_decl_name cparams exp_cparams extern_params params
     start_state states
     ⊣ Γ <| cnstrs :=
             parser_decl_name
-              ↦ ParserType
-              (map snd cparams) expr_cparams
+              ↦ CtrType Cnstr.Parser
+              (map snd cparams) exp_cparams
               (map snd extern_params) params ,, cnstrs Γ |>
 | type_extern
-    extern_name type_params cparams expr_cparams methods :
-  (* TODO: check types as [t_ok] *)
-  Γ ⊢tp TopDecl.Extern extern_name type_params cparams expr_cparams methods
+    extern_name type_params cparams exp_cparams methods :
+  (* TODO: check types as [typ_ok] *)
+  Γ ⊢tp Top.Extern extern_name type_params cparams exp_cparams methods
     ⊣ Γ <| cnstrs :=
               extern_name
                 ↦ ExternType
                 type_params (map snd cparams)
-                expr_cparams extern_name ,, cnstrs Γ |>
+                exp_cparams extern_name ,, cnstrs Γ |>
 | type_function function_name type_params arrow body sig :
   good_signal arrow sig ->
   `⧼ type_params, bind_all (paramargs arrow) [], tfuncts Γ,
       CFunction (rtrns arrow) ⧽ ⊢ body ⊣ sig ->
-  Γ ⊢tp TopDecl.Funct
+  Γ ⊢tp Top.Funct
     function_name type_params arrow body
     ⊣ Γ <| tfuncts := function_name ↦ (type_params,arrow) ,, tfuncts Γ |>
 where
 "Γ₁ '⊢tp' d ⊣ Γ₂"
-  := (type_topdecl Γ₁ d Γ₂).
+  := (type_top Γ₁ d Γ₂).
 
 Local Close Scope climate_scope.
 
 Definition type_prog
-  : TopDecl.prog -> top_type_env -> top_type_env -> Prop :=
+  : Top.prog -> top_type_env -> top_type_env -> Prop :=
   FoldLeft (fun d Γ Γ' => Γ ⊢tp d ⊣ Γ').
