coq/lib/GCL/V1model.v
@@ -8,10 +8,10 @@ Module G := GCL.GCL.
 Module F := GCL.Form.
 Module BV := GCL.BitVec.
 Module E := GCL.E.
-Module ST := Stmt.
+Module ST := Stm.
 
 Definition externs : ToGCL.model :=
-  [("_", [("mark_to_drop",  G.GAssign (E.TBit (BinNat.N.of_nat 9)) "standard_metadata.egress_spec" (BV.bit (Some 9%nat) 511));
+  [("_", [("mark_to_drop",  G.GAssign (Typ.Bit (BinNat.N.of_nat 9)) "standard_metadata.egress_spec" (BV.bit (Some 9%nat) 511));
          ("clone3", G.GSkip);
          ("assert", G.GAssert (F.LVar "check"));
          ("assume", G.GAssume (F.LVar "check"));
@@ -21,7 +21,7 @@ Definition externs : ToGCL.model :=
          ("crc_poly", G.GSkip);
          ("digest", G.GSkip)
    ]);
-  ("packet_in", [("extract", G.GAssign (E.TBit 1%N) "hdr.is_valid" (BV.bit (Some 1%nat) 1))]);
+  ("packet_in", [("extract", G.GAssign (Typ.Bit 1%N) "hdr.is_valid" (BV.bit (Some 1%nat) 1))]);
   ("counter", [("count", G.GSkip)]);
   ("direct_counter", [("count", G.GSkip)]);
   ("register", [("read", G.GSkip); ("write", G.GSkip)]);
@@ -29,44 +29,44 @@ Definition externs : ToGCL.model :=
   ("direct_meter", [("direct_meter", G.GSkip); ("read", G.GSkip)])
   ].
 
-Definition cub_seq (statements : list ST.s): ST.s :=
+Definition cub_seq (statements : list ST.t): ST.t :=
   List.fold_right ST.Seq ST.Skip statements.
 
 Definition det_fwd_asst   :=
   let assertion :=
-      E.Bop E.TBool
-             E.NotEq
-             (E.Var (E.TBit 9%N) "standard_metadata.egress_spec" 0)
+      E.Bop Typ.Bool
+             Bin.NotEq
+             (E.Var (Typ.Bit 9%N) "standard_metadata.egress_spec" 0)
              (E.Bit 9%N 0%Z)
   in
   let paramargs := [(*check*) PAIn assertion] in
-  ST.Call (ST.Method "_" "assert" [] None) paramargs.
+  ST.App (Call.Method "_" "assert" [] None) paramargs.
 
-Definition standard_metadata_t : Expr.t :=
-  Expr.TStruct
+Definition standard_metadata_t : Typ.t :=
+  Typ.Struct
     false
-    [Expr.TBit 9 (*ingress_port*);
-     Expr.TBit 9 (*egress_spec*);
-     Expr.TBit 9 (*egress_port*);
-     Expr.TBit 32 (*instance_type*);
-     Expr.TBit 32 (*packet_length*);
-     Expr.TBit 32 (*enq_timestamp*);
-     Expr.TBit 19 (*enq_qdepth*);
-     Expr.TBit 32 (*deq_timedelta*);
-     Expr.TBit 19 (*deq_qdepth*);
-     Expr.TBit 48 (*ingress_global_timestamp*);
-     Expr.TBit 48 (*egress_global_timestamp*);
-     Expr.TBit 16 (*mcast_grp*);
-     Expr.TBit 16 (*egress_rid*);
-     Expr.TBit 1 (*checksum_error*);
-     Expr.TError (* parser error *);
-     Expr.TBit 3 (*priority*)].
+    [Typ.Bit 9 (*ingress_port*);
+     Typ.Bit 9 (*egress_spec*);
+     Typ.Bit 9 (*egress_port*);
+     Typ.Bit 32 (*instance_type*);
+     Typ.Bit 32 (*packet_length*);
+     Typ.Bit 32 (*enq_timestamp*);
+     Typ.Bit 19 (*enq_qdepth*);
+     Typ.Bit 32 (*deq_timedelta*);
+     Typ.Bit 19 (*deq_qdepth*);
+     Typ.Bit 48 (*ingress_global_timestamp*);
+     Typ.Bit 48 (*egress_global_timestamp*);
+     Typ.Bit 16 (*mcast_grp*);
+     Typ.Bit 16 (*egress_rid*);
+     Typ.Bit 1 (*checksum_error*);
+     Typ.Error (* parser error *);
+     Typ.Bit 3 (*priority*)].
 
 (* TODO: correct de bruijn index? *)
-Definition t_arg (dir : E.e -> paramarg E.e E.e) typ var :=
+Definition t_arg (dir : E.t -> paramarg E.t E.t) typ var :=
   (var, dir (E.Var typ var 0)).
 
-Definition pipeline  (htype mtype : E.t) (parser v_check ingress egress c_check deparser : string) : ST.s  :=
+Definition pipeline  (htype mtype : Typ.t) (parser v_check ingress egress c_check deparser : string) : ST.t  :=
   let ext_args := ["packet_in"] in
   let pargs := [
         t_arg PAOut      htype                "parsedHdr";
@@ -89,13 +89,13 @@ Definition pipeline  (htype mtype : E.t) (parser v_check ingress egress c_check 
   let dep_ext_args := [ "packet_out" ; "b" ] in
   let dep_args := [ t_arg PAIn htype "hdr"] in
   cub_seq [
-        ST.Apply parser  ext_args (map snd pargs) ;
+        ST.App (Call.Inst parser ext_args) (map snd pargs) ;
           (* ST.Apply v_check ext_args vck_args i; *)
-          ST.Conditional
-            (E.Var E.TBool ("_state$accept$next") 0)
+          ST.Cond
+            (E.Var Typ.Bool ("_state$accept$next") 0)
             (cub_seq [
-                       ST.Apply ingress ext_args (map snd ing_args)
-                       ; ST.Apply egress  ext_args (map snd egr_args)
+                       ST.App (Call.Inst ingress ext_args) (map snd ing_args)
+                       ; ST.App (Call.Inst egress ext_args) (map snd egr_args)
                        ; det_fwd_asst
             ])
             ST.Skip
@@ -103,7 +103,7 @@ Definition pipeline  (htype mtype : E.t) (parser v_check ingress egress c_check 
         (* ST.Apply   deparser ext_args dep_args NoInfo *)
     ].
 
-Definition package (types : list E.t) (cargs : TopDecl.constructor_args) : result string ST.s :=
+Definition package (types : list Typ.t) (cargs : Top.constructor_args) : result string ST.t :=
   match cargs with
   | [p; vc; ing; egr; cc; d] =>
     match types with
@@ -119,7 +119,7 @@ Definition package (types : list E.t) (cargs : TopDecl.constructor_args) : resul
   end.
 
 Definition gcl_from_p4cub instr gas unroll p4cub : result string ToGCL.target :=
-  let arrowtype := ({|paramargs:=[("check", PAIn E.TBool)]; rtrns:=None|} : Expr.arrowT) in
-  let assume_decl := TopDecl.Extern "_" 1 [] [] [("assume", (0%nat, [], arrowtype))] in
+  let arrowtype := ({|paramargs:=[("check", PAIn Typ.Bool)]; rtrns:=None|} : Typ.arrowT) in
+  let assume_decl := Top.Extern "_" 1 [] [] [("assume", (0%nat, [], arrowtype))] in
   let p4cub_instrumented := ToP4cub.add_extern  p4cub assume_decl in
   ToGCL.from_p4cub  instr gas unroll externs (package) p4cub.
